

Mateo Toro

$$\overline{T}_{00} = T_{00} \left(\frac{-12d\vec{i} + 5d\vec{k}}{\sqrt{(12d)^2 + (5d)^2}} \right) = T_{00} \left(\frac{-12}{13} \vec{i} + \frac{5}{13} \vec{k} \right)$$

$$\overline{T_{BE}} = T_{BE} \left(\frac{-12\vec{i} + 5\vec{j}}{\sqrt{(-12a)^2 + (5a)^2}} \right) = T_{BE} \left(\frac{-12}{13} \vec{i} + \frac{5}{13} \vec{j} \right)$$

$$\overline{T_{cu}} = T_{cu} \left(\frac{-12d\vec{i} + 3d\vec{j} - 4d\vec{k}}{\sqrt{(-12d)^2 + (3d)^2 + (-4d)^2}} \right) = T_{cu} \left(-\frac{12}{13} \vec{i} + \frac{3}{13} \vec{j} - \frac{4}{13} \vec{k} \right)$$

Moment Equilibrium About Point O

$$\sum \bar{M}_O = 0 = [\bar{r}_{Oc} \times \bar{T}_{cH}] + [\bar{r}_{On} \times \bar{T}_{BE}] + [\bar{r}_{On} \times \bar{T}_{Bo}] + [\bar{r}_{Oc} \times \bar{F}_c] + [\bar{r}_{On} \times \bar{F}_o]$$

$$\bar{r}_{Oc} \times \bar{T}_{cH} = \begin{vmatrix} 12d & 0 & 0 \\ -\frac{12}{13} & \frac{3}{13} & -\frac{4}{13} \end{vmatrix} = \frac{48}{13} d \hat{j} + \frac{36}{13} d \hat{k} \quad \bullet \quad T_{cH}$$

$$\bar{r}_{On} \times \bar{T}_{BE} = \begin{vmatrix} 12d & 0 & 6d \\ -\frac{12}{13} & \frac{5}{13} & 0 \end{vmatrix} = -\frac{36}{13} d \hat{i} - \frac{72}{13} d \hat{j} + \frac{60}{13} d \hat{k} \quad \bullet \quad T_{BE}$$

$$\bar{r}_{On} \times \bar{T}_{Bo} = \begin{vmatrix} 12d & 0 & 6d \\ -\frac{12}{13} & 0 & \frac{5}{13} \end{vmatrix} = -\left(\frac{60}{13} d - \left(-\frac{72}{13} d\right)\right) \hat{j} = -\frac{132}{13} d \hat{j} \quad \bullet \quad T_{Bo}$$

$$\bar{r}_{Oc} \times \bar{F}_c = \begin{vmatrix} 12d & 0 & 0 \\ 0 & -P & 0 \end{vmatrix} = -12dP \hat{k}$$

$$\bar{r}_{On} \times \bar{F}_B = \begin{vmatrix} 12d & 0 & 6d \\ 0 & -P & 0 \end{vmatrix} = 6Fd \hat{i} - 12Fd \hat{k}$$

$$\begin{aligned} \sum \bar{M}_O = 0 &= T_{cH} \frac{48}{13} d \hat{j} + T_{cH} \frac{36}{13} d \hat{k} - T_{BE} \frac{36}{13} d \hat{i} - T_{BE} \frac{72}{13} d \hat{j} + T_{BE} \frac{60}{13} d \hat{k} \\ &- T_{Bo} \frac{132}{13} d \hat{j} - 12Fd \hat{k} + 6Fd \hat{i} - 12Fd \hat{k} \end{aligned}$$

Sum of moments in components

$$\sum M_x = 0 = -T_{BE} \frac{36}{13} d + 6Fd$$

$$\rightarrow T_{BE} = 6Fd \left(\frac{13}{36d} \right)$$

$$T_{BE} = \frac{13}{5} F \quad \text{or} \quad 2.6 F$$

$$\sum M_z = 0 = T_{CH} \frac{36}{13} d + T_{BE} \frac{60}{13} d - 12Fd - 12Fd$$

$$0 = T_{CH} \frac{36}{13} d + \left(\frac{13}{5} F \right) \frac{60}{13} d - 12Fd - 12Fd$$

$$0 = T_{CH} \frac{36}{13} d + 12Fd - 12Fd - 12Fd$$

$$T_{CH} \frac{36}{13} d = 12Fd$$

$$\rightarrow T_{CH} = 12Fd \left(\frac{13}{36d} \right)$$

$$T_{CH} = \frac{13}{3} F \quad \text{or} \quad 4.33 F$$

$$\sum M_y = 0 = T_{CH} \frac{48}{13} d - T_{BE} \frac{72}{13} d - T_{BD} \frac{132}{13} d$$

$$0 = \left(\frac{13}{3} F \right) \frac{48}{13} d - \left(\frac{13}{5} F \right) \frac{72}{13} d - T_{BD} \frac{132}{13} d$$

$$0 = 16Fd - \frac{72}{5} Fd - T_{BD} \frac{132}{13} d$$

$$T_{BD} \frac{132}{13} d = \frac{8}{5} Fd$$

$$\rightarrow T_{BD} = \frac{8}{5} Fd \left(\frac{13}{132d} \right)$$

$$T_{BD} = \frac{26}{125} F \quad \text{or} \quad 0.158 F$$